---
title: "Influence function calculation for Brier score for event time data"
author: "Johan Sebastian Ohlendorff & Thomas Alexander Gerds"
date: "2022-06-07"
output:
  pdf_document: default
  word_document: default
header-includes: \usepackage{graphicx, verbatim, fancyvrb, setspace, xspace, colortbl,
  longtable, amsmath, caption, xfrac, float, mathabx,bbm,algorithm2e}
---



\newcommand{\Xj}{\ensuremath{X^{\prime}}}
\newcommand{\xj}{\ensuremath{x^{\prime}}}
\newcommand{\AUC}{\ensuremath{\operatorname{AUC}}}
\newcommand{\Brier}{\ensuremath{\operatorname{Brier}}}
\newcommand{\survtau}{\ensuremath{\tilde S(\tau)}}
\newcommand{\hatsurvtau}{\ensuremath{\hat{\tilde{S}}(\tau)}}
\newcommand{\Htau}{\ensuremath{H(\tau)}}
\newcommand{\hatHtau}{\ensuremath{\hat H^{(i)}(\tau)}}

\newcommand{\Utau}{\ensuremath{U(\tau)}}
\newcommand{\hatUtau}{\ensuremath{\hat U^{(i)}(\tau)}}
\newcommand{\Vtau}{\ensuremath{V(\tau)}}
\newcommand{\hatVtau}{\ensuremath{\hat V^{(i)}(\tau)}}
\newcommand{\Wtau}{\ensuremath{W(\tau)}}
\newcommand{\hatWtau}{\ensuremath{\hat W^{(i)}(\tau)}}
\newcommand{\margprob}{\ensuremath{F}}
\newcommand{\hatmargprob}{\ensuremath{\hat{F}}}
\newcommand{\Zi}{\ensuremath{Z_i}}
\newcommand{\emp}{\ensuremath{I\negthickspace P_n}}
\newcommand{\ifauc}{\ensuremath{\mathrm{IF}_{\mathrm{AUC}}}}
\newcommand{\hatifauc}{\ensuremath{\mathrm{\widehat{IF}}_{\mathrm{AUC}}}}
\newcommand{\ifnu}{\ensuremath{\mathrm{IF}_{\nu}}}
\newcommand{\ifnuc}{\ensuremath{\mathrm{IF}^1_{\nu}}}
\newcommand{\hatifnu}{\ensuremath{\mathrm{\widehat{IF}}_{\nu}}}
\newcommand{\hatifnuc}{\ensuremath{\mathrm{\widehat{IF}}^1_{\nu}}}
\newcommand{\ifmu}{\ensuremath{\mathrm{IF}_{\mu}}}
\newcommand{\hatifmu}{\ensuremath{\mathrm{\widehat{IF}}_{\mu}}}
\newcommand{\ifmuc}{\ensuremath{\mathrm{IF}^1_{\mu}}}
\newcommand{\hatifmuc}{\ensuremath{\mathrm{\widehat{IF}}^1_{\mu}}}

% for use with Rikkes paper
\newcommand{\AUCO}{\hat{\theta}^{(1,1)}_{\tau,m}}
\newcommand{\auc}{\widehat{\text{auc}}}
\newcommand{\aucO}{\theta_{\tau,m}}
\newcommand{\D}{\mathrm{d}}
\newcommand{\Db}{D^*_{m,b}}
\newcommand{\E}{\mathbb{E}}
\newcommand{\G}{\hat G_n}
\newcommand{\g}{\hat{\mathbb{G}}}
\newcommand{\II}{\mathcal{I}}
\newcommand{\I}[1]{\II_{\{#1\}}}
\newcommand{\Ibi}{\I{N_i^b=0}}
\newcommand{\Ibj}{\I{N_j^b=0}}
\newcommand{\Ibk}{\I{N_k^b=0}}
\newcommand{\IC}{\text{IF}}
\newcommand{\Isi}{\I{N_i=0}}
\newcommand{\LL}{\{\I{\T_{m+1}\leq \tau}-\R(Z_{m+1})\}^2}
\newcommand{\Lbi}{\{\I{\T_i\leq \tau}-\Rb(Z_i)\}^2}
\newcommand{\Li}{\{\I{\T_i\leq \tau}-\R(Z_i)\}^2}
\newcommand{\Lj}{\{\I{\T_j\leq \tau}-\R(Z_j)\}^2}
\newcommand{\loo}{leave-one-out bootstrap }
\newcommand{\lpo}{leave-pair-out bootstrap }
\newcommand{\Lt}{\ensuremath{L_t}}
\newcommand{\M}{\ensuremath{\omega_{\tau,m}}}
\newcommand{\m}{\hat{\omega}^{(1)}_{\tau,m}}
\newcommand{\mbin}{\hat{\omega}^{(1)}_{m}}
\newcommand{\MU}{\ensuremath{\hat{\mu}^{(1)}_{\tau,m}}}
\newcommand{\p}{\ensuremath{\P_n}}
\newcommand{\PSI}{\ensuremath{\hat{\psi}^{(1)}_{m}}}
\renewcommand{\P}{\ensuremath{\mathrm{P}}}
\newcommand{\PEK}{\ensuremath{P_{\epsilon,k}}}
\newcommand{\Qej}{\ensuremath{Q_{n,\epsilon,j}}}
\newcommand{\RR}{\ensuremath{R_{\tau}}}
\newcommand{\R}{\ensuremath{\RR(D_m)}}
\newcommand{\Rb}{\ensuremath{\RR(D_{m,b}^*)}}
\newcommand{\Rbi}{\ensuremath{R(D_{m,b}^*)}}
\newcommand{\T}{\ensuremath{\tilde{T}}}
\newcommand{\V}{\text{Var}}
\newcommand{\X}{\ensuremath{\tilde{X}}}
\newcommand{\XX}{X}
\newcommand{\W}{W_\tau}
\newcommand{\Wi}{\W(X_i,\hat G_n)}
\newcommand{\Wk}{\W(X_k,\hat G_n)}
\newcommand{\WWi}{\mathcal{W}_{T_i}(Z_i)}
\newcommand{\WWj}{\mathcal{W}_t(Z_j)}

```{r setup, include=FALSE}
knitr::opts_chunk$set(echo = TRUE)
```

## IF Calculation
To describe the situation with competing risks (and also survival) we introduce a
random variable \(D\in\{1,2\}\) which indicates the cause (i.e., type
of the event) observed at time \(T\) such that \(D=1\) means that the
event of interest occurred, and \(D=2\) that a competing risk
occurred. As in the survival setting we let \(Q\) denote the joint
probability measure of the uncensored data, \((T,D,X)\sim Q\), and $P$
the joint probability measure of the right censored data
$Z=(\tilde{T},\Delta,X) \sim P$ now with $\Delta=D 1_{\{T \leq C\}}$
taking values in the set \(\{0,1,2\}\). We are interested in the
following definition of the time-dependent discrimination measure for
cause 1. We can easily calculate the influence function for the Brier score, which can be written as: 
\begin{align*}
& \int\left\{1_{\{ t \leq \tau \}}-R(\tau \mid x)\right\}^{2} Q(d t, d x)\\
&=\int 1_{\{t \leqslant \tau\}}-21_{\{t \leqslant \tau\}} R(\tau \mid x)+R(\tau \mid x)^{2} Q(d t, d x) \\
&= \int 1_{\{t \leqslant \tau\}}(1-2 R(\tau \mid x)) Q(d t, d x)+\int R(\tau \mid x)^{2} Q(d x) \\
&=\int \frac{1_{\{t \leqslant \tau\}}}{G(t- |x)}(1-2 R(\tau \mid x)) P(d t, 1, d x) + \int R\left(\tau | x\right)^2 P(d x)
\end{align*}
We find
\begin{align*}
IC_{\Brier}(\tilde{T}_i,\Delta_i,X_i;\tau) &= \partial_{\varepsilon} \int \frac{1_{\{t \leqslant \tau\}}}{G(t- |x)}(1-2 R(\tau \mid x)) P_{\varepsilon}(d t, 1, d x) +\partial_{\varepsilon} \int R\left(\tau | x\right)^2 P_{\varepsilon}(d x) \\&=
\int 1_{\{t \leqslant \tau \}}(1-2 R(\tau \mid x)) \frac{d(\delta_{\left\{\tilde{T}_{i}, \Delta_i,X_i\right\}})(t, 1, x)+dP(t,1,x)\left[f_i(t-,x)-1\right]}{G(t- |x)} \\
&+ \int R\left(\tau | x\right)^2 (\delta_{\left\{\tilde{T}_{i}, \Delta_i,X_i\right\}}-P) \\
&=   1_{\{\tilde{T}_i \leqslant \tau, \Delta_i=1\}}(1-2 R(\tau \mid X_i)) \frac{1}{G(\tilde{T}_i- | X_i)}  \\
&+  \int 1_{\{t \leqslant \tau\}}(1-2 R(\tau \mid x)) f_i(t-,x) \frac{dP(t,1,x)}{G(t-|x)} + R\left(\tau | X_i \right)^2 \\
&- \int R\left(\tau | x\right)^2 dP(x)
- \int 1_{\{t \leqslant \tau\}}(1-2 R(\tau \mid x)) \frac{dP(t,1,x)}{G(t-|x)}
\end{align*}
The last term that is subtracted is the Brier score. Then using that 
$$
 f_i(t,x) = \frac{\mathbbm{1}_{\{\tilde{T_i} \leq t, \Delta_i = 0\}} \delta_{X_i}(x)}{G(\tilde{T_i}|X_i)S(\tilde{T_i}|X_i)} -\int_0^{\tilde{T}_i \wedge t} \frac{ \delta_{X_i}(x)dP(s,0 | x)}{G(s|X_i)^2S(s|X_i)^2}
$$
we see that (plugging in $f(t,x)$ instead of $f(t-,x)$!)
$$
\begin{aligned}
\int_X \int_0^\tau(1-2R(\tau|x))f_i(t-,x) \frac{P(dt,1,x)}{G(t-|x)} &= \int_X \int_0^\tau(1-2R(\tau|x))\left[\frac{\mathbbm{1}_{\{\tilde{T_i} \leq t, \Delta_i = 0\}} \delta_{X_i}(x)}{G(\tilde{T_i}|X_i)S(\tilde{T_i}|X_i)} -\int_0^{\tilde{T}_i \wedge t} \frac{ \delta_{X_i}(x)P(ds,0 | x)}{G(s|X_i)^2S(s|X_i)^2}\right] \frac{P(dt,1,x)}{G(t-|x)} \\
&= \int_0^\tau(1-2R(\tau|X_i))\left[\frac{\mathbbm{1}_{\{\tilde{T_i} \leq t, \Delta_i = 0\}} }{G(\tilde{T_i}|X_i)S(\tilde{T_i}|X_i)} -\int_0^{\tilde{T}_i \wedge t} \frac{ P(ds,0 | X_i)}{G(s|X_i)^2S(s|X_i)^2}\right] \frac{P(dt,1 | X_i)}{G(t-|X_i)} \\
&= (i) - (ii)
\end{aligned}
$$
where 
$$
\begin{aligned}
(i) &=\int_0^\tau(1-2R(\tau|X_i))\frac{\mathbbm{1}_{\{\tilde{T_i} \leq t, \Delta_i = 0\}} }{G(\tilde{T_i}|X_i)S(\tilde{T_i}|X_i)} \frac{P(dt,1 | X_i)}{G(t-|X_i)} \\
&= (1-2R(\tau|X_i))\frac{\mathbbm{1}_{\{\tilde{T}_i \leq \tau,\Delta_i = 0\}} }{G(\tilde{T_i}|X_i)S(\tilde{T_i}|X_i)} \int_{\tilde{T}_i}^\tau \frac{P(dt,1 | X_i)}{G(t-|X_i)} \\
&= (1-2R(\tau|X_i))\frac{\mathbbm{1}_{\{\tilde{T}_i \leq \tau,\Delta_i = 0\}} }{G(\tilde{T_i}|X_i)S(\tilde{T_i}|X_i)} (F_1(\tau|X_i)-F_1(\tilde{T}_i|X_i))
\end{aligned}
$$

Similarly, we have
$$
\begin{aligned}
(ii) &=(1-2R(\tau|X_i))\int_0^\tau\int_0^{\tilde{T}_i \wedge t} \frac{ P(ds,0 | X_i)}{G(s|X_i)^2S(s|X_i)^2} \frac{P(dt,1 | X_i)}{G(t-|X_i)} \\
\end{aligned}
$$
If $\tilde{T}_i > \tau$, then this can be written as 
$$
\begin{aligned}
(ii) &=(1-2R(\tau|X_i))\int_0^\tau\int_s^{\tau} \frac{ P(dt,1 | X_i)}{G(t-|X_i)} \frac{P(ds,0 | X_i)}{G(s|X_i)^2S(s|X_i)^2} \\
&= (1-2R(\tau|X_i))\int_0^\tau(F_1(\tau|X_i)-F_1(s|X_i)) \frac{P(ds,0 | X_i)}{G(s|X_i)^2S(s|X_i)^2} 
\end{aligned}
$$
On the other hand, if $\tilde{T}_i \leq \tau$, then
$$
\begin{aligned}
(ii) &=(1-2R(\tau|X_i))\int_0^{\tilde{T}_i}\int_s^{\tau} \frac{ P(dt,1 | X_i)}{G(t-|X_i)} \frac{P(ds,0 | X_i)}{G(s|X_i)^2S(s|X_i)^2}  \\
&= (1-2R(\tau|X_i))\int_0^{\tilde{T}_i}(F_1(\tau|X_i)-F_1(s|X_i)) \frac{P(ds,0 | X_i)}{G(s|X_i)^2S(s|X_i)^2} 
\end{aligned}
$$
Thus 
$$
\begin{aligned}
(ii) 
&= (1-2R(\tau|X_i))\int_0^{\tilde{T}_i \wedge \tau}(F_1(\tau|X_i)-F_1(s|X_i)) \frac{P(ds,0 | X_i)}{G(s|X_i)^2S(s|X_i)^2} 
\end{aligned}
$$
Hence, 
$$
(i)-(ii) = (1-2R(\tau |X_i))\left(\frac{I(\tilde{T}_i \leq \tau, \Delta_i = 0)}{G(\tilde{T}_i|X_i)S(\tilde{T}_i|X_i)}(F_1(\tau|X_i)-F_1(\tilde{T}_i|X_i))-\int_0^{\tilde{T}_i \wedge \tau} \frac{(F_1(\tau|X_i)-F_1(s|X_i))}{G(s|X_i)^2S(s|X_i)^2}P(ds,0|X_i)\right)
$$


## Not expanding the paranthesis
We can also derive the Brier score as:
\begin{align*}
\sum_{\delta = 0, 1} \int\left\{1_{\{ t \leq \tau \}}-R(\tau \mid x)\right\}^{2} W_\tau(z; G) P(d t, \delta, d x)
\end{align*}
with $W_\tau(z; G) = \frac{\delta I(t \leq \tau)}{G(t-|x)} +  \frac{I(t > \tau)}{G(\tau |x)}$. Taking the Gateaux derivative yields,
\begin{align*}
& I( \tilde{T}_i \leq \tau, \Delta_i=1)\frac{(1-R(\tau \mid X_i)) ^{2}}{G(\tilde{T}_i- | X_i)} + I( \tilde{T}_i > \tau)\frac{R(\tau \mid X_i) ^{2}}{G(\tau | X_i)} \\
&-Brier \\
&+ \int I(t \leq \tau)(1-R(\tau | x))^2 \frac{f_i(t-,x)}{G(t-|x)}P(dt,1,dx) \\
&+ \int I(t > \tau)R(\tau | x) ^2 \frac{f_i(\tau,x)}{G(\tau|x)}P(dt,dx)
\end{align*}
Whenever the censoring does not depend on covariates, the two last integrals are easy to estimate. However, when the censoring does depend on the covariates, we can use the tricks mentioned in IFAUC.pdf to get that,
\begin{align*}
&\int I(t > \tau)R(\tau | x) ^2 \frac{f_i(\tau,x)}{G(\tau|x)}P(dt,dx) + \int I(t \leq \tau)(1-R(\tau | x))^2 \frac{f_i(t-,x)}{G(t-|x)}P(dt,1,dx) \\
&= R(\tau | X_i)^2 S(\tau | X_i)\left(\frac{I(\tilde{T}_i \leq \tau, \Delta_i = 0)}{G(\tilde{T}_i|X_i)S(\tilde{T}_i|X_i)}-\int_0^{\tilde{T}_i \wedge \tau} \frac{1}{G(s|X_i)^2S(s|X_i)^2}P(ds,0|X_i)\right) \\
&+ (1-R(\tau|X_i))^2 \left(\frac{I(\tilde{T}_i \leq \tau, \Delta_i = 0)}{G(\tilde{T}_i|X_i)S(\tilde{T}_i|X_i)}(F_1(\tau|X_i)-F_1(\tilde{T}_i|X_i))-\int_0^{\tilde{T}_i \wedge \tau} \frac{(F_1(\tau|X_i)-F_1(s|X_i))}{G(s|X_i)^2S(s|X_i)^2}P(ds,0|X_i)\right) \\
&= R(\tau | X_i)^2 S(\tau | X_i)\left(\frac{I(\tilde{T}_i \leq \tau, \Delta_i = 0)}{G(\tilde{T}_i|X_i)S(\tilde{T}_i|X_i)}-\int_0^{\tilde{T}_i \wedge \tau} \frac{1}{G(s|X_i)S(s|X_i)}\Lambda_C(ds|X_i)\right) \\
&+ (1-R(\tau|X_i))^2 \left(\frac{I(\tilde{T}_i \leq \tau, \Delta_i = 0)}{G(\tilde{T}_i|X_i)S(\tilde{T}_i|X_i)}(F_1(\tau|X_i)-F_1(\tilde{T}_i|X_i))-\int_0^{\tilde{T}_i \wedge \tau} \frac{(F_1(\tau|X_i)-F_1(s|X_i))}{G(s|X_i)S(s|X_i)}\Lambda_C(ds|X_i)\right)
\end{align*}

## IF with cross-validation

### Binary case
Our cross-validation algorithm repeatedly splits the dataset \(D_n\) of size $n$
into training and validation datasets as follows. Let \(B\) be a large
integer. For each \(b=1,\ldots,B\) we draw a bootstrap dataset
\(\Db=\{X_{b,1}^*,\ldots,X_{b,m}^*\}\) of size \(m\) with
replacement from the data \(D_n\). For \(i=1,\ldots,n\) let \(N_i^b\) be
the number of times subject \(i\) is included in \(\Db\). In step
\(b\) of the cross-validation algorithm the bootstrap dataset \(\Db\)
is used for training. We apply \(R \) to \(\Db\) to obtain the
prediction model \(\Rbi\). All subjects \(i\) for which \(N_i^b=0\) are
out-of-bag and we let these subjects form the validation dataset of step \(b\). First let us construct the influence function in this case with binary data, $X=(Y,Z)$. In this case, we consider estimation of the functional (i.e. the definition of the Brier score in cross-validation)

\begin{align*}
  \psi_{m}(P)&=\int\left(\int\cdots\int\left\{y_{m+1}-R(\{x_i\}_{i=1}^m)(z_{m+1})\right\}^2 I(x_{m+1} \notin \{x_i\}_{i=1}^m)\prod_{i=1}^m P(d x_i)\right) P(d x_{m+1}) 
\end{align*}

for some sample size $m < n$. Let 
\begin{equation*}
  \omega_{m} (Y_{m+1},Z_{m+1})=\mathbb{E}_{D_m} [(Y_{m+1}-R(D_m)(Z_{m+1}))^2 | Y_{m+1}, Z_{m+1}] 
\end{equation*}
because then $\psi_{m}(P) = \mathbb{E}_{X_{m+1}}[\omega_{m} (Y_{m+1},Z_{m+1})]$. For estimating $\omega_{\tau,m}$, we propose to use leave one-out bootstrap estimation:
\begin{equation*}
  \hat{\omega}_{m} (Y_i,Z_i)=\frac{\sum_{b=1}^B (Y_{i}-R(D_m)(Z_{i}))^2I(N_i^b=0) }{\sum_{b=1}^B I(N_i^b=0)}
\end{equation*}
Finally, the Brier score may then be estimated by leave one-out bootstrap estimation as Â´
\begin{equation*}
  \PSI=\frac{1}{n}\sum_{i=1}^n\hat{\omega}_{m} (Y_i,Z_i)
\end{equation*}
Finally, we also want standard errors of the estimates. For this, we consider the influence function by taking the Gateaux derivative and get: 
\begin{align*} 
  \IC_{\psi}(m;x_k)&=\frac{\partial}{\partial\epsilon}\psi_{m}(P_{\epsilon,k})\Big\vert_{\epsilon=0} \\
  &= \int \frac{\partial}{\partial\epsilon} \left(\int\cdots\int\left\{y_{m+1}-R(\{x_i\}_{i=1}^m)(z_{m+1})\right\}^2 I(x_{m+1} \notin \{x_i\}_{i=1}^m)\prod_{i=1}^m \PEK (d x_i)\right) \PEK(d x_{m+1}) \Big\vert_{\epsilon=0} \\
  &= \int \frac{\partial}{\partial\epsilon} \left(\int\cdots\int\left\{y_{m+1}-R(\{x_i\}_{i=1}^m)(z_{m+1})\right\}^2 I(x_{m+1} \notin \{x_i\}_{i=1}^m)\prod_{i=1}^m \PEK (d x_i)\right) \Big\vert_{\epsilon=0}  P(d x_{m+1}) \\
  &+  \int \left(\int\cdots\int\left\{y_{m+1}-R(\{x_i\}_{i=1}^m)(z_{m+1})\right\}^2 I(x_{m+1} \notin \{x_i\}_{i=1}^m)\prod_{i=1}^m P (d x_i)\right) \frac{\partial}{\partial\epsilon} \PEK(d x_{m+1}) \Big\vert_{\epsilon=0}  \\
  &= \int \sum_{j=1}^m \left(\int\cdots\int\left\{y_{m+1}-R(\{x_i\}_{i=1}^m)(z_{m+1})\right\}^2 I(x_{m+1} \notin \{x_i\}_{i=1}^m) \delta_{x_k}(x_j) \prod_{i \neq j} (d x_i)\right)  P(d x_{m+1})  - m \psi_{m}(P) \\ %notation???
  &+ \omega_{m} (Y_{k},Z_{k})-\psi_{m}(P) \\
  &= \omega_{m} (Y_{k},Z_{k})-(m+1) \psi_{m}(P) \\
  &+\int \sum_{j=1}^m \left(\int\cdots\int\left\{y_{m+1}-R(\{x_i\}_{i=1}^m)(z_{m+1})\right\}^2 I(x_{m+1} \notin \{x_i\}_{i=1}^m) \delta_{x_k}(x_j) \prod_{i \neq j} (d x_i)\right)  P(d x_{m+1}) 
\end{align*}
wherein we used the product rule of differentiation. For estimating the influence function, we suggest the estimator:
\begin{align*}
  \widehat{\IC}_{\psi}(m;X_k)&=\mbin (Y_k,Z_k)-(m+1)\, \PSI +\frac{1}{n} \sum_{i=1}^n\frac{\sum_b \{Y_i-\Rbi (Z_i)\}^2 \Ibi N_k^b}{\sum_b\Ibi} % is the last part estimated correctly?
\end{align*}

### Survival and competing risk case
Let us now try to expand this to the case with (right-censored) survival data, i.e. $X=(T, \Delta, Z)$ and let $\bar{X} = (\tilde{T},Z)$ denote the true event time, i.e. $T=\min\{\tilde{T}, C\}$ and $\Delta = I(T\leq C)$, where $C$ is the censoring time. Also let $Y_i = I(\tilde{T} \leq \tau)$ (or $T$, depending on whichever is the most appropriate), where $\tau$ be some prespecified time point and \(\G\) be an estimate of the censoring
distribution \(G\) based on \(D_n\). Then we are concerned with the functional $\mu_{\tau, m}$ 
\begin{equation*}
  \mu_{\tau,m}=\E_{\X_{m+1}}\big[\E_{D_{m}}\big[\LL\big|\T_{m+1},Z_{m+1}\big]\big]
\end{equation*} 
By rewriting the above above a bit (i.e. by using standard tricks when rewriting in terms of the observed data), it can be shown that this quantity can be defined in terms of the observed data, i.e. it can be expressed as the value of
a statistical functional \(\psi_{\tau,m}:\mathcal{P}\to [0,1]\)
\begin{align*}
  \psi_{\tau,m}(\P)&=\int\left(\int\cdots\int\left\{\I{u_{m+1}\leq\tau}-\RR(\{x_i\}_{i=1}^m)(z_{m+1})\right\}^2 I(x_{m+1} \notin \{x_i\}_{i=1}^m) \prod_{i=1}^m\P(\D x_i)\right)\\
   &\qquad\qquad\times\W(x_{m+1},\kappa_{\tau,z_{m+1}}(\P))\P(\D x_{m+1})\\&=\mu_{\tau,m}.
\end{align*}
with 
\begin{align*}
  \Wi=\frac{\I{T_i\leq \tau}\Delta_i}{\G(T_i\vert Z_i)}+\frac{\I{T_i>\tau}}{\G(\tau\vert Z_i)}
\end{align*} 
then this can be estimated in much the same way as before, i.e. as 
\begin{equation*}
  \MU=\frac{1}{n}\sum_{i=1}^n\m(T_i,Z_i)\Wi 
\end{equation*}
Here, we redefine that 
\begin{equation*}
  \m(\T_i,Z_i)=\frac{\sum_{b=1}^B\Lbi\Ibi}{\sum_{b=1}^B\I{N_i^b=0}}
\end{equation*}
In much the same way as before, we may find the the influence function of $\psi_{\tau,m}(\P)$ to be almost the same as before with an additional term corresponding to the fact that the censoring distribution has to be estimated, i.e. 
\begin{align*} 
  \IC_{\psi}(\tau,m;x_k)&=\M(t_k,z_k)\W(x_k,\kappa_{\tau,z_{m+1}}(\P))-(m+1)\, \mu_{\tau,m}\\
  &+\int\Big[\sum_{j=1}^m \int\cdots\int\{\I{t_{m+1}\leq\tau}-\RR(\{x_i\}_{i=1}^n)(z_{m+1})\}^2 I(x_{m+1} \notin \{x_i\}_{i=1}^m) \delta_{x_k}(x_j)\prod_{i\neq j}\P(\D x_i)\Big]\W(x_{m+1},\kappa_{\tau,z_{m+1}}(\P))\P(\D x_{m+1})
  \\
  &+\int\M(t_{m+1},z_{m+1})\left[\frac{\I{t_{m+1}\leq \tau}\delta_{m+1}}{G(t_{m+1}-\vert z_{m+1})} f_k(t_{m+1},z_{m+1})
  +\frac{\I{t_{m+1}>\tau}}{G(\tau\vert z_{m+1})}f_k(\tau,z_{m+1}) \right]\P(\D x_{m+1}) \\
\end{align*}
This can then be estimated in much the same way as before
\begin{align*}
  \widehat{\IC}_{\psi}(\tau,m;X_k)&=\m(T_k,Z_k)\W(X_k,\G)-(m+1)\, \MU \\
  &+\frac{1}{n} \sum_{i=1}^n\frac{\sum_b \{\I{T_i\leq \tau}-\Rb(Z_i)\}^2 \Ibi N_k^b}{\sum_b\Ibi}\W(X_i,\G)\\
  &+\frac{1}{n}\sum_{i=1}^n\m(T_i,Z_i)\left[\frac{\I{T_i\leq\tau}\Delta_i}{\G(T_i-\vert Z_i)}\hat{f_k} (T_i-,Z_i)
  +\frac{\I{T_i>\tau}}{\G (\tau\vert Z_i)}\hat{f_k} (\tau ,Z_i)\right]
\end{align*}
Here the last term corresponds to the censoring being unknown. 